cachelessScript.sml
@@ -435,6 +435,109 @@ val cl_fixmmu_Tr_oblg = store_thm("cl_fixmmu_Tr_oblg", ``
 		 coreIfTheory.Tr__def]
 );
 
+(********* bisimulation properties *********)
+
+val deps_MD_lem = store_thm("deps_MD_lem", ``
+!s sc. (s.cs = sc.cs)
+    /\ (!pa. pa IN ca_deps sc ==> (cl_Cv s (MEM pa) = Cv sc (MEM pa)))
+        ==>
+    (!r. r IN MDVA sc (ca_vdeps sc) ==> (cl_Cv s r = Cv sc r))
+``,
+  RW_TAC std_ss [cl_Cv_def, Cv_def] >>
+  ASSUME_TAC ( SPEC ``r:resource`` coreIfTheory.res_cases ) >>
+  FULL_SIMP_TAC std_ss []
+  >| [(* MEM pa *)
+      FULL_SIMP_TAC std_ss [] >>
+      IMP_RES_TAC ca_deps_MD_oblg >>
+      RES_TAC >>
+      METIS_TAC []
+      ,
+      (* register *)
+      Cases_on `r` >> (
+          FULL_SIMP_TAC std_ss [coreIfTheory.reg_res_def, coreIfTheory.CV_def]
+      )
+     ]
+);
+
+val deps_vdeps_eq_lem = store_thm("deps_vdeps_eq_lem", ``
+!s sc. (s.cs = sc.cs)
+    /\ (!pa. pa IN ca_deps sc ==> (cl_Cv s (MEM pa) = Cv sc (MEM pa)))
+        ==>
+    (cl_vdeps s = ca_vdeps sc)
+``,
+  RW_TAC std_ss [cl_vdeps_def, ca_vdeps_def]
+);
+
+val deps_MD_eq_lem = store_thm("deps_MD_eq_lem", ``
+!s sc. (s.cs = sc.cs)
+    /\ (!pa. pa IN ca_deps sc ==> (cl_Cv s (MEM pa) = Cv sc (MEM pa)))
+        ==>
+    (cl_MDVA s (cl_vdeps s) = MDVA sc (ca_vdeps sc))
+``,
+  REPEAT STRIP_TAC >>
+  IMP_RES_TAC deps_vdeps_eq_lem >>
+  IMP_RES_TAC deps_MD_lem >>
+  FULL_SIMP_TAC  std_ss [cl_MDVA_def, MDVA_def, cl_Cv_def, Cv_def] >>
+  MATCH_MP_TAC EQ_SYM >>
+  MATCH_MP_TAC MD__lem >>
+  REPEAT STRIP_TAC >>
+  RES_TAC >>
+  REV_FULL_SIMP_TAC std_ss [] 
+);
+
+val deps_Tr_eq_lem = store_thm("deps_Tr_eq_lem", ``
+!s sc. (s.cs = sc.cs)
+    /\ (!pa. pa IN ca_deps sc ==> (cl_Cv s (MEM pa) = Cv sc (MEM pa)))
+        ==>
+    (!va. va IN ca_vdeps sc ==> (cl_Tr s va = ca_Tr sc va))
+``,
+  REPEAT STRIP_TAC >>
+  IMP_RES_TAC deps_vdeps_eq_lem >>
+  IMP_RES_TAC deps_MD_lem >>
+  `MDVA sc (ca_vdeps sc) = cl_MDVA s (cl_vdeps s)` by (
+      IMP_RES_TAC deps_MD_eq_lem >>
+      FULL_SIMP_TAC std_ss []
+  ) >>
+  FULL_SIMP_TAC  std_ss [cl_MDVA_def, MDVA_def, cl_Cv_def, Cv_def, 
+			 cl_Tr_def, ca_Tr_def, coreIfTheory.Tr__def] >>
+  MATCH_MP_TAC (
+      prove(``(x = y) ==> (FST x = FST y)``, PROVE_TAC [])
+  ) >>
+  MATCH_MP_TAC (
+      prove(``(x = y) ==> (THE x = THE y)``, PROVE_TAC [])
+  ) >>
+  `va IN cl_vdeps s` by ( RW_TAC std_ss [] ) >>
+  IMP_RES_TAC Mmu_lem >>
+  REV_FULL_SIMP_TAC std_ss []  
+);
+
+val deps_eq_oblg = store_thm("deps_eq_oblg", ``
+!s sc. (s.cs = sc.cs)
+    /\ (!pa. pa IN ca_deps sc ==> (cl_Cv s (MEM pa) = Cv sc (MEM pa)))
+        ==>
+    (cl_deps s = ca_deps sc)
+``,
+  REPEAT STRIP_TAC >>
+  IMP_RES_TAC deps_MD_eq_lem >>
+  IMP_RES_TAC deps_Tr_eq_lem >>
+  FULL_SIMP_TAC std_ss [cl_deps_def, ca_deps_def, cl_Cv_def, Cv_def, 
+			MDVA_def, cl_MDVA_def, coreIfTheory.deps__def,
+		        pred_setTheory.IN_UNION] >>
+  MATCH_MP_TAC (
+      prove(``(A = C) /\ (B = D) ==> (A UNION B = C UNION D)``, PROVE_TAC [])
+  ) >>
+  RW_TAC std_ss [pred_setTheory.EXTENSION]
+  >| [(* vdeps *)
+      FULL_SIMP_TAC std_ss [cl_Tr_def, ca_Tr_def, ca_vdeps_def,
+			    pred_setTheory.IN_GSPEC_IFF] >>
+      METIS_TAC []
+      ,
+      (* MD *)
+      FULL_SIMP_TAC std_ss [cl_vdeps_def, ca_vdeps_def,
+			    pred_setTheory.IN_GSPEC_IFF] >>
+      REV_FULL_SIMP_TAC std_ss []
+     ]
+);
 
 (********* cacheless computation **********)
 
